<?xml version="1.0"?>
<rdf:RDF xmlns="https://w3id.org/polifonia/ontology/music-analysis/"
     xml:base="https://w3id.org/polifonia/ontology/music-analysis/"
     xmlns:dc="http://purl.org/dc/elements/1.1/"
     xmlns:mr="https://w3id.org/polifonia/ontology/music-representation/"
     xmlns:ns="http://creativecommons.org/ns#"
     xmlns:owl="http://www.w3.org/2002/07/owl#"
     xmlns:rdf="http://www.w3.org/1999/02/22-rdf-syntax-ns#"
     xmlns:xml="http://www.w3.org/XML/1998/namespace"
     xmlns:xsd="http://www.w3.org/2001/XMLSchema#"
     xmlns:core="https://w3id.org/polifonia/ontology/core/"
     xmlns:rdfs="http://www.w3.org/2000/01/rdf-schema#"
     xmlns:skos="http://www.w3.org/2004/02/skos/core#"
     xmlns:vann="http://purl.org/vocab/vann/"
     xmlns:dcterms="http://purl.org/dc/terms/">
    <owl:Ontology rdf:about="https://w3id.org/polifonia/ontology/music-analysis">
        <owl:imports rdf:resource="https://w3id.org/polifonia/ontology/core/"/>
        <owl:imports rdf:resource="https://w3id.org/polifonia/ontology/music-representation/"/>
        <ns:licence rdf:resource="https://creativecommons.org/licenses/by-sa/4.0/"/>
        <dcterms:creator xml:lang="en">Nicolas Lazzari</dcterms:creator>
        <dcterms:description xml:lang="en">The Music Analysis ontology implements different musical theories that are used by expert to analyse musical composition. Each theory extends the rudiments defined by the Music Projection module.

The music analysis module acts as an hub that imports all the different theories, implemented as submodules.</dcterms:description>
        <dcterms:issued xml:lang="en">30/07/2023</dcterms:issued>
        <dcterms:license rdf:resource="https://creativecommons.org/licenses/by-sa/4.0/"/>
        <dcterms:modified xml:lang="en">30/07/2023</dcterms:modified>
        <dcterms:rights rdf:resource="https://creativecommons.org/licenses/by-sa/4.0/"/>
        <dcterms:title xml:lang="en">Music Analysis Ontology</dcterms:title>
        <vann:preferredNamespacePrefix>ma:</vann:preferredNamespacePrefix>
        <vann:preferredNamespaceUri rdf:resource="https://w3id.org/polifonia/ontology/music-analysis/"/>
        <rdfs:comment xml:lang="en">The Music Analysis ontology implements different musical theories that are used by expert to analyse musical composition. Each theory extends the rudiments defined by the Music Projection module.

The music analysis module acts as an hub that imports all the different theories, implemented as submodules.</rdfs:comment>
        <rdfs:isDefinedBy xml:lang="en">Polifonia Ontology Network</rdfs:isDefinedBy>
        <rdfs:label>Music Analysis Ontology</rdfs:label>
        <owl:versionInfo xml:lang="en">1.0</owl:versionInfo>
    </owl:Ontology>
    


    <!-- 
    ///////////////////////////////////////////////////////////////////////////////////////
    //
    // Object Properties
    //
    ///////////////////////////////////////////////////////////////////////////////////////
     -->

    


    <!-- https://w3id.org/polifonia/ontology/music-analysis/definesProjection -->

    <owl:ObjectProperty rdf:about="https://w3id.org/polifonia/ontology/music-analysis/definesProjection">
        <rdfs:subPropertyOf rdf:resource="https://w3id.org/polifonia/ontology/core/defines"/>
    </owl:ObjectProperty>
    


    <!-- 
    ///////////////////////////////////////////////////////////////////////////////////////
    //
    // Classes
    //
    ///////////////////////////////////////////////////////////////////////////////////////
     -->

    


    <!-- https://w3id.org/polifonia/ontology/music-analysis/TheoryContribution -->

    <owl:Class rdf:about="https://w3id.org/polifonia/ontology/music-analysis/TheoryContribution">
        <rdfs:subClassOf>
            <owl:Restriction>
                <owl:onProperty rdf:resource="https://w3id.org/polifonia/ontology/core/hasAgent"/>
                <owl:someValuesFrom rdf:resource="https://w3id.org/polifonia/ontology/core/Agent"/>
            </owl:Restriction>
        </rdfs:subClassOf>
        <rdfs:subClassOf>
            <owl:Restriction>
                <owl:onProperty rdf:resource="https://w3id.org/polifonia/ontology/core/hasAgentRole"/>
                <owl:someValuesFrom rdf:resource="https://w3id.org/polifonia/ontology/core/AgentRole"/>
            </owl:Restriction>
        </rdfs:subClassOf>
        <rdfs:subClassOf>
            <owl:Restriction>
                <owl:onProperty rdf:resource="https://w3id.org/polifonia/ontology/core/hasAgent"/>
                <owl:allValuesFrom rdf:resource="https://w3id.org/polifonia/ontology/core/Agent"/>
            </owl:Restriction>
        </rdfs:subClassOf>
        <rdfs:subClassOf>
            <owl:Restriction>
                <owl:onProperty rdf:resource="https://w3id.org/polifonia/ontology/core/hasAgentRole"/>
                <owl:allValuesFrom rdf:resource="https://w3id.org/polifonia/ontology/core/AgentRole"/>
            </owl:Restriction>
        </rdfs:subClassOf>
        <rdfs:comment>Situation where an agent contribute to the definition, formalisation or interpretation of a musical theory.</rdfs:comment>
        <rdfs:label>Theory Contribution</rdfs:label>
    </owl:Class>
    


    <!-- https://w3id.org/polifonia/ontology/music-representation/AnalyticalReference -->

    <rdf:Description rdf:about="https://w3id.org/polifonia/ontology/music-representation/AnalyticalReference">
        <rdfs:subClassOf>
            <owl:Restriction>
                <owl:onProperty rdf:resource="https://w3id.org/polifonia/ontology/core/defines"/>
                <owl:someValuesFrom rdf:resource="https://w3id.org/polifonia/ontology/music-representation/MusicProjection"/>
            </owl:Restriction>
        </rdfs:subClassOf>
        <rdfs:subClassOf>
            <owl:Restriction>
                <owl:onProperty rdf:resource="https://w3id.org/polifonia/ontology/core/defines"/>
                <owl:allValuesFrom rdf:resource="https://w3id.org/polifonia/ontology/music-representation/MusicProjection"/>
            </owl:Restriction>
        </rdfs:subClassOf>
        <rdfs:subClassOf>
            <owl:Restriction>
                <owl:onProperty rdf:resource="https://w3id.org/polifonia/ontology/core/involvesAgent"/>
                <owl:allValuesFrom rdf:resource="https://w3id.org/polifonia/ontology/music-analysis/TheoryContribution"/>
            </owl:Restriction>
        </rdfs:subClassOf>
    </rdf:Description>
    


    <!-- 
    ///////////////////////////////////////////////////////////////////////////////////////
    //
    // Individuals
    //
    ///////////////////////////////////////////////////////////////////////////////////////
     -->

    


    <!-- https://w3id.org/polifonia/ontology/music-analysis -->

    <owl:NamedIndividual rdf:about="https://w3id.org/polifonia/ontology/music-analysis">
        <rdf:type rdf:resource="http://purl.org/vocab/vann/Vocabulary"/>
    </owl:NamedIndividual>
</rdf:RDF>



<!-- Generated by the OWL API (version 4.5.25.2023-02-15T19:15:49Z) https://github.com/owlcs/owlapi -->

